verified/nlarith.s.dfy
@@ -1,0 +1,9 @@
+lemma {:axiom} lemma_MulModZero(a:int, b:int)
+    requires b > 0
+    ensures (a * b) % b == 0
+/* FIXME: prove this! */
+
+lemma lemma_DivMulLessThan(a:int, b:int)
+    requires b > 0
+    ensures (a / b) * b <= a
+{}
