verified/subdir.mk
@@ -1,4 +1,4 @@
-DAFNYFLAGS = /noNLarith /timeLimit:60 /trace
+DAFNYFLAGS = /timeLimit:60 /trace
 SPARTANFLAGS = #-assumeUpdates 1
 
 # top-level target
@@ -23,11 +23,14 @@ mkincs-nodir = $(call mkdfyincs,$(1),) $(call mksdfyincs,$(1),)
 # Spartan direct verification, including cheesy workaround for broken error code.
 %.verified %.log: %.sdfy %.gen.dfy
 	/bin/bash -c "$(SPARTAN) $(SPARTANFLAGS) $(call mkincs-dir,$*) $< \
-	-dafnyDirect $(DAFNYFLAGS) /compile:0 | tee $*.log; exit \$${PIPESTATUS[0]}"
+	-dafnyDirect $(DAFNYFLAGS) /noNLarith /compile:0 | tee $*.log; exit \$${PIPESTATUS[0]}"
 	@grep -q "^Dafny program verifier finished with [^0][0-9]* verified, 0 errors$$" $*.log && touch $*.verified
 	@$(RM) $*.log
 
 %.verified: %.dfy
+	$(DAFNY) $(DAFNYFLAGS) /noNLarith /compile:0 $< && touch $@
+
+$(dir)/nlarith.s.verified: $(dir)/nlarith.s.dfy
 	$(DAFNY) $(DAFNYFLAGS) /compile:0 $< && touch $@
 
 %.exe: %.i.dfy %.i.verified
@@ -50,6 +53,7 @@ CLEAN := $(CLEAN) $(dir)/*.exe $(dir)/*.dll $(dir)/*.pdb $(dir)/*.S $(dir)/*.o $
 
 # deps for all Dafny code
 $(dir)/ARMdef.verified: $(dir)/Maybe.verified $(dir)/Seq.verified $(dir)/bitvectors.s.verified
+$(dir)/bitvectors.s.verified: $(dir)/nlarith.s.verified
 $(dir)/ARMprint.verified: $(dir)/ARMdef.verified
 $(dir)/ARMspartan.verified: $(dir)/ARMdef.verified
 $(dir)/kom_common.s.verified: $(dir)/ARMdef.verified
